Optimize proof RUs (#56)
* Decrease RU usage in model.dfy

* Hide `InstanceOfRequestType`, `InstanceOfEntityTypeStore`, and `InstanceOfActionStore`

Placing these common preconditions in an opaque predicate reduces RU
usage in the lemmas that don't need to know the internals of each
predicate. The change brings two proofs under the 10,000,000 RU limit,
with the highest RU proof dropping from 23.9M to 14.7M

* reduced RU of SoundCall

---------

Co-authored-by: Shaobo He <shaobohe@amazon.com>

cedar-dafny/validation/thm/soundness.dfy
@@ -76,6 +76,10 @@ module validation.thm.soundness {
       WellTyped(e,effs) && subty(getType(e, effs), t)
     }
 
+    ghost predicate {:opaque} WellFormedRequestAndStore() {
+      InstanceOfRequestType(r,reqty) && InstanceOfEntityTypeStore(s,ets) && InstanceOfActionStore(s,acts)
+    }
+
     // On input to the typechecking function, for any (e,k) in the Effects,
     // e is a record- or entity-typed expression that has key k.
     ghost predicate {:opaque} EffectsInvariant (effs: Effects) {
@@ -120,13 +124,12 @@ module validation.thm.soundness {
 
     lemma SoundVar(x: Var, t: Type, effs: Effects)
       decreases Var(x) , 0
-      requires InstanceOfRequestType(r,reqty)
-      requires InstanceOfEntityTypeStore(s,ets)
-      requires InstanceOfActionStore(s,acts)
+      requires WellFormedRequestAndStore()
       requires Typesafe(Var(x),effs,t)
       ensures IsSafe(r,s,Var(x),t)
       ensures getEffects(Var(x),effs) == Effects.empty()
     {
+      assert InstanceOfRequestType(r, reqty) by { reveal WellFormedRequestAndStore(); }
       var t' :| getType(Var(x),effs) == t' && subty(t',t);
       assert Typechecker(ets,acts,reqty).inferVar(x) == types.Ok(t');
       match x {
@@ -186,9 +189,7 @@ module validation.thm.soundness {
 
     lemma SoundIf(e: Expr, e1: Expr, e2: Expr, t: Type, effs: Effects)
       decreases If(e,e1,e2) , 0
-      requires InstanceOfRequestType(r,reqty)
-      requires InstanceOfEntityTypeStore(s,ets)
-      requires InstanceOfActionStore(s,acts)
+      requires WellFormedRequestAndStore()
       requires EffectsInvariant(effs)
       requires Typesafe(If(e,e1,e2),effs,t)
       ensures IsSafe(r,s,If(e,e1,e2),t)
@@ -326,9 +327,7 @@ module validation.thm.soundness {
 
     lemma SoundAnd(e1: Expr, e2: Expr, t: Type, effs: Effects)
       decreases And(e1,e2) , 0
-      requires InstanceOfRequestType(r,reqty)
-      requires InstanceOfEntityTypeStore(s,ets)
-      requires InstanceOfActionStore(s,acts)
+      requires WellFormedRequestAndStore()
       requires EffectsInvariant(effs)
       requires Typesafe(And(e1,e2),effs,t)
       ensures IsSafe(r,s,And(e1,e2),t)
@@ -463,9 +462,7 @@ module validation.thm.soundness {
 
     lemma SoundOr(e1: Expr, e2: Expr, t: Type, effs: Effects)
       decreases Or(e1,e2) , 0
-      requires InstanceOfRequestType(r,reqty)
-      requires InstanceOfEntityTypeStore(s,ets)
-      requires InstanceOfActionStore(s,acts)
+      requires WellFormedRequestAndStore()
       requires EffectsInvariant(effs)
       requires Typesafe(Or(e1,e2),effs,t)
       ensures IsSafe(r,s,Or(e1,e2),t)
@@ -579,9 +576,7 @@ module validation.thm.soundness {
 
     lemma SoundNot(e: Expr, t: Type, effs: Effects)
       decreases UnaryApp(Not,e) , 0
-      requires InstanceOfRequestType(r,reqty)
-      requires InstanceOfEntityTypeStore(s,ets)
-      requires InstanceOfActionStore(s,acts)
+      requires WellFormedRequestAndStore()
       requires EffectsInvariant(effs)
       requires Typesafe(UnaryApp(Not,e),effs,t)
       ensures IsSafe(r,s,UnaryApp(Not,e),t)
@@ -608,9 +603,7 @@ module validation.thm.soundness {
 
     lemma SoundNeg(e: Expr, t: Type, effs: Effects)
       decreases UnaryApp(Neg,e) , 0
-      requires InstanceOfRequestType(r,reqty)
-      requires InstanceOfEntityTypeStore(s,ets)
-      requires InstanceOfActionStore(s,acts)
+      requires WellFormedRequestAndStore()
       requires EffectsInvariant(effs)
       requires Typesafe(UnaryApp(Neg,e),effs,t)
       ensures IsSafe(r,s,UnaryApp(Neg,e),t)
@@ -630,9 +623,7 @@ module validation.thm.soundness {
 
     lemma SoundMulBy(i: int, e: Expr, t: Type, effs: Effects)
       decreases UnaryApp(MulBy(i),e) , 0
-      requires InstanceOfRequestType(r,reqty)
-      requires InstanceOfEntityTypeStore(s,ets)
-      requires InstanceOfActionStore(s,acts)
+      requires WellFormedRequestAndStore()
       requires EffectsInvariant(effs)
       requires Typesafe(UnaryApp(MulBy(i),e),effs,t)
       ensures IsSafe(r,s,UnaryApp(MulBy(i),e),t)
@@ -652,9 +643,7 @@ module validation.thm.soundness {
 
     lemma SoundLike(e: Expr, p: Pattern, t: Type, effs: Effects)
       decreases UnaryApp(Like(p),e) , 0
-      requires InstanceOfRequestType(r,reqty)
-      requires InstanceOfEntityTypeStore(s,ets)
-      requires InstanceOfActionStore(s,acts)
+      requires WellFormedRequestAndStore()
       requires EffectsInvariant(effs)
       requires Typesafe(UnaryApp(Like(p),e),effs,t)
       ensures IsSafe(r,s,UnaryApp(Like(p),e),t)
@@ -722,9 +711,7 @@ module validation.thm.soundness {
 
     lemma SoundEq(e1: Expr, e2: Expr, t: Type, effs: Effects)
       decreases BinaryApp(BinaryOp.Eq,e1,e2) , 0
-      requires InstanceOfRequestType(r,reqty)
-      requires InstanceOfEntityTypeStore(s,ets)
-      requires InstanceOfActionStore(s,acts)
+      requires WellFormedRequestAndStore()
       requires EffectsInvariant(effs)
       requires Typesafe(BinaryApp(BinaryOp.Eq,e1,e2),effs,t)
       ensures IsSafe(r,s,BinaryApp(BinaryOp.Eq,e1,e2),t)
@@ -747,6 +734,7 @@ module validation.thm.soundness {
             EqFalseIsSafe(r,s,e1,e2,t1.lub,t2.lub);
           } else if Typechecker(ets,acts,reqty).isUnspecifiedVar(e1) && t2.Entity? && t2.lub.specified() {
             assert t' == Type.Bool(False);
+            reveal WellFormedRequestAndStore();
             UnspecifiedVarHasUnspecifiedEntityType(e1);
             EqFalseIsSafe(r,s,e1,e2,unspecifiedEntityType.lub,t2.lub);
           } else {
@@ -763,9 +751,7 @@ module validation.thm.soundness {
     lemma SoundIneq(op: BinaryOp, e1: Expr, e2: Expr, t: Type, effs: Effects)
       decreases BinaryApp(op,e1,e2) , 0
       requires op == Less || op == BinaryOp.LessEq
-      requires InstanceOfRequestType(r,reqty)
-      requires InstanceOfEntityTypeStore(s,ets)
-      requires InstanceOfActionStore(s,acts)
+      requires WellFormedRequestAndStore()
       requires EffectsInvariant(effs)
       requires Typesafe(BinaryApp(op,e1,e2),effs,t)
       ensures IsSafe(r,s,BinaryApp(op,e1,e2),t)
@@ -789,9 +775,7 @@ module validation.thm.soundness {
     lemma SoundArith(op: BinaryOp, e1: Expr, e2: Expr, t: Type, effs: Effects)
       decreases BinaryApp(op,e1,e2) , 0
       requires op == Add || op == Sub
-      requires InstanceOfRequestType(r,reqty)
-      requires InstanceOfEntityTypeStore(s,ets)
-      requires InstanceOfActionStore(s,acts)
+      requires WellFormedRequestAndStore()
       requires EffectsInvariant(effs)
       requires Typesafe(BinaryApp(op,e1,e2),effs,t)
       ensures IsSafe(r,s,BinaryApp(op,e1,e2),t)
@@ -815,9 +799,7 @@ module validation.thm.soundness {
     lemma SoundContainsAnyAll(op: BinaryOp, e1: Expr, e2: Expr, t: Type, effs: Effects)
       decreases BinaryApp(op,e1,e2) , 0
       requires op == ContainsAny || op == ContainsAll
-      requires InstanceOfRequestType(r,reqty)
-      requires InstanceOfEntityTypeStore(s,ets)
-      requires InstanceOfActionStore(s,acts)
+      requires WellFormedRequestAndStore()
       requires EffectsInvariant(effs)
       requires Typesafe(BinaryApp(op,e1,e2),effs,t)
       ensures IsSafe(r,s,BinaryApp(op,e1,e2),t)
@@ -840,9 +822,7 @@ module validation.thm.soundness {
 
     lemma SoundContains(e1: Expr, e2: Expr, t: Type, effs: Effects)
       decreases BinaryApp(Contains,e1,e2) , 0
-      requires InstanceOfRequestType(r,reqty)
-      requires InstanceOfEntityTypeStore(s,ets)
-      requires InstanceOfActionStore(s,acts)
+      requires WellFormedRequestAndStore()
       requires EffectsInvariant(effs)
       requires Typesafe(BinaryApp(Contains,e1,e2),effs,t)
       ensures IsSafe(r,s,BinaryApp(Contains,e1,e2),t)
@@ -872,9 +852,7 @@ module validation.thm.soundness {
 
     lemma SoundRecord(es: seq<(Attr,Expr)>, t: Type, effs: Effects)
       decreases Expr.Record(es) , 0
-      requires InstanceOfRequestType(r,reqty)
-      requires InstanceOfEntityTypeStore(s,ets)
-      requires InstanceOfActionStore(s,acts)
+      requires WellFormedRequestAndStore()
       requires EffectsInvariant(effs)
       requires Typesafe(Expr.Record(es),effs,t)
       ensures IsSafe(r,s,Expr.Record(es),t)
@@ -944,9 +922,7 @@ module validation.thm.soundness {
 
     lemma SoundSet(es: seq<Expr>, t: Type, effs: Effects)
       decreases Expr.Set(es) , 0
-      requires InstanceOfRequestType(r,reqty)
-      requires InstanceOfEntityTypeStore(s,ets)
-      requires InstanceOfActionStore(s,acts)
+      requires WellFormedRequestAndStore()
       requires Typesafe(Expr.Set(es),effs,t)
       requires EffectsInvariant(effs)
       ensures IsSafe(r,s,Expr.Set(es),t)
@@ -974,9 +950,7 @@ module validation.thm.soundness {
 
     lemma SoundGetAttr(e: Expr, k: Attr, t: Type, effs: Effects)
       decreases GetAttr(e,k) , 0
-      requires InstanceOfRequestType(r,reqty)
-      requires InstanceOfEntityTypeStore(s,ets)
-      requires InstanceOfActionStore(s,acts)
+      requires WellFormedRequestAndStore()
       requires EffectsInvariant(effs)
       requires Typesafe(GetAttr(e,k),effs,t)
       ensures IsSafe(r,s,GetAttr(e,k),t)
@@ -1021,6 +995,7 @@ module validation.thm.soundness {
               ensures rt.attrs[k].isRequired ==> k in s.entities[euid].attrs
               ensures k in s.entities[euid].attrs ==> InstanceOfType(s.entities[euid].attrs[k],t')
             {
+              reveal WellFormedRequestAndStore();
               GetLubRecordTypeSubty(lub, euid.ty);
               SubtyCompat(ets.types[euid.ty].attrs[k].ty, t');
             }
@@ -1051,6 +1026,7 @@ module validation.thm.soundness {
       assert !rtl.isOpen() ==> rt1.attrs.Keys == rt2.attrs.Keys;
 
       LubRecordType(rt1, rt2);
+      reveal WellFormedRequestAndStore();
 
       forall k | k in rtl.attrs.Keys
         ensures subtyAttrType(rt1.attrs[k], rtl.attrs[k]) && subtyAttrType(rt2.attrs[k], rtl.attrs[k]) {
@@ -1098,9 +1074,7 @@ module validation.thm.soundness {
 
     lemma SoundHasAttr(e: Expr, k: Attr, t: Type, effs: Effects)
       decreases HasAttr(e,k) , 0
-      requires InstanceOfRequestType(r,reqty)
-      requires InstanceOfEntityTypeStore(s,ets)
-      requires InstanceOfActionStore(s,acts)
+      requires WellFormedRequestAndStore()
       requires EffectsInvariant(effs)
       requires Typesafe(HasAttr(e,k),effs,t)
       ensures IsSafe(r,s,HasAttr(e,k),t)
@@ -1159,6 +1133,7 @@ module validation.thm.soundness {
           assert Typesafe(e,effs,Type.Entity(et)) by { SubtyRefl(Type.Entity(et)); }
           assert IsSafe(r,s,e,Type.Entity(et)) by { Sound(e,Type.Entity(et),effs); }
           if !ets.isAttrPossible(et,k) {
+            reveal WellFormedRequestAndStore();
             EntityHasImpossibleFalseSafe(r,s,e,k,et);
           } else {
             var m := ets.getLubRecordType(et).value;
@@ -1216,9 +1191,7 @@ module validation.thm.soundness {
 
     lemma SoundInSetMemberFalse(e1: Expr, ei2s: seq<Expr>, i: nat, effs: Effects)
       decreases BinaryApp(BinaryOp.In,e1,Expr.Set(ei2s)) , 0 , Expr.Set(ei2s) , 0
-      requires InstanceOfRequestType(r,reqty)
-      requires InstanceOfEntityTypeStore(s,ets)
-      requires InstanceOfActionStore(s,acts)
+      requires WellFormedRequestAndStore()
       requires EffectsInvariant(effs)
       requires WellTyped(BinaryApp(BinaryOp.In,e1,Expr.Set(ei2s)),effs)
       requires getType(BinaryApp(BinaryOp.In,e1,Expr.Set(ei2s)),effs) == Type.Bool(False)
@@ -1246,6 +1219,7 @@ module validation.thm.soundness {
           assert t1 == Type.Entity(EntityLUB({et1}));
           assert IsSafe(r,s,Var(v1),t1) by { Sound(e1,t1,effs); }
           assert !ets.possibleDescendantOf(et1,u2.ty);
+          reveal WellFormedRequestAndStore();
           InSingleFalseEntityTypeAndLiteral(r,s,e1,et1,u2);
         case PrimitiveLit(EntityUID(u1)) =>
           if isAction(u1.ty) {
@@ -1255,15 +1229,14 @@ module validation.thm.soundness {
             assert !ets.possibleDescendantOfSet(u1.ty,ets2);
             assert !ets.possibleDescendantOf(u1.ty,u2.ty);
           }
+          reveal WellFormedRequestAndStore();
           InSingleFalseLiterals(r,s,u1,u2);
       }
     }
 
     lemma SoundIn(e1: Expr, e2: Expr, t: Type, effs: Effects)
       decreases BinaryApp(BinaryOp.In,e1,e2) , 0 , e2
-      requires InstanceOfRequestType(r,reqty)
-      requires InstanceOfEntityTypeStore(s,ets)
-      requires InstanceOfActionStore(s,acts)
+      requires WellFormedRequestAndStore()
       requires EffectsInvariant(effs)
       requires Typesafe(BinaryApp(BinaryOp.In,e1,e2),effs,t)
       ensures IsSafe(r,s,BinaryApp(BinaryOp.In,e1,e2),t)
@@ -1295,6 +1268,7 @@ module validation.thm.soundness {
       match t' {
         // Easy case
         case Bool(AnyBool) =>
+          reveal WellFormedRequestAndStore();
           assert IsSafe(r,s,BinaryApp(BinaryOp.In,e1,e2),Type.Bool(AnyBool)) by {
             if e2IsSet {
               assert IsSafe(r,s,e2,Type.Set(Type.Entity(AnyEntity))) by { Sound(e2,Type.Set(Type.Entity(AnyEntity)),effs); }
@@ -1307,6 +1281,7 @@ module validation.thm.soundness {
         // Harder case: we have to prove that the result is false.
         case Bool(False) =>
           if typechecker.isUnspecifiedVar(e1) && e2IsSpecified {
+            reveal WellFormedRequestAndStore();
             UnspecifiedVarHasUnspecifiedEntityType(e1);
             assert IsSafe(r,s,e2,t2) by { Sound(e2,t2,effs); }
             if e2IsSet {
@@ -1323,6 +1298,7 @@ module validation.thm.soundness {
                   assert t1 == Type.Entity(EntityLUB({et1}));
                   assert IsSafe(r,s,Var(v1),t1) by { Sound(e1,t1,effs); }
                   assert !ets.possibleDescendantOf(et1,u2.ty);
+                  reveal WellFormedRequestAndStore();
                   InSingleFalseEntityTypeAndLiteral(r,s,e1,et1,u2);
                 case PrimitiveLit(EntityUID(u1)) =>
                   if isAction(u1.ty) {
@@ -1330,6 +1306,7 @@ module validation.thm.soundness {
                   } else {
                     assert !ets.possibleDescendantOf(u1.ty,u2.ty);
                   }
+                  reveal WellFormedRequestAndStore();
                   InSingleFalseLiterals(r,s,u1,u2);
               }
               case Set(ei2s) =>
@@ -1373,19 +1350,29 @@ module validation.thm.soundness {
       ensures forall i | 0 <= i < |args| :: Typesafe(args[i],effs,tys[i])
     {}
 
+    lemma TypesafeCallSemantics(name: base.Name, es: seq<Expr>, effs: Effects, t: Type)
+    requires Typesafe(Call(name,es),effs,t)
+    ensures name in extFunTypes
+    ensures |extFunTypes[name].args| == |es|
+    ensures forall i | 0 <= i < |es| :: Typesafe(es[i],effs,extFunTypes[name].args[i])
+    ensures extFunTypes[name].ret == t
+    {
+      assert Typechecker(ets,acts,reqty).inferCall(Call(name,es),name,es,effs).Ok?;
+      InferCallArgsSound(Call(name,es),name,es,extFunTypes[name].args,effs);
+    }
+
+
     lemma SoundCall(name: base.Name, es: seq<Expr>, t: Type, effs: Effects)
       decreases Call(name,es) , 0
-      requires InstanceOfRequestType(r,reqty)
-      requires InstanceOfEntityTypeStore(s,ets)
-      requires InstanceOfActionStore(s,acts)
+      requires WellFormedRequestAndStore()
       requires EffectsInvariant(effs)
       requires Typesafe(Call(name,es),effs,t)
       ensures IsSafe(r,s,Call(name,es),t)
       ensures getEffects(Call(name,es),effs) == Effects.empty()
     {
       assert Typechecker(ets,acts,reqty).inferCall(Call(name,es),name,es,effs).Ok?;
+      TypesafeCallSemantics(name, es, effs, t);
       var eft := extFunTypes[name];
-      InferCallArgsSound(Call(name,es),name,es,eft.args,effs);
       forall i | 0 <= i < |es| ensures IsSafe(r,s,es[i],eft.args[i]) {
         Sound(es[i],eft.args[i],effs);
       }
@@ -1394,9 +1381,7 @@ module validation.thm.soundness {
 
     lemma Sound(e: Expr, t: Type, effs: Effects)
       decreases e , 1
-      requires InstanceOfRequestType(r,reqty)
-      requires InstanceOfEntityTypeStore(s,ets)
-      requires InstanceOfActionStore(s,acts)
+      requires WellFormedRequestAndStore()
       requires EffectsInvariant(effs)
       requires Typesafe(e,effs,t)
       ensures IsSafe(r,s,e,t)
@@ -1440,6 +1425,7 @@ module validation.thm.soundness {
       ensures IsSafe(r,s,e,t)
     {
       EmptyEffectsInvariant();
+      reveal WellFormedRequestAndStore();
       Sound(e,t,Effects.empty());
     }
   }
